L: lambda
A: App

FokkerChallenge/EncoderDecoder/Basic.lean
@@ -12,116 +12,67 @@ namespace Cslib
 namespace LambdaCalculus.LocallyNameless.Untyped.Term
 
 
--- 2. Encoder (Modified to return Option (List Bool))
-def encodeVar : Nat → List Bool
-  | 0 => [true, false]
-  | n + 1 => true :: encodeVar n
+@[simp, scoped grind =]
+def lt7: Term String -> Bool
+  | Term.bvar n => n < 7
+  | Term.fvar _ => true
+  | Term.abs t => lt7 t
+  | Term.app t1 t2 => lt7 t1 && lt7 t2
 
-def encode: Term String → Option (List Bool)
-  | Term.bvar i => some (encodeVar i)
+@[simp, scoped grind =]
+def encode: Term String → Option (List Char)
+  | Term.bvar 0 => some (['0'])
+  | Term.bvar 1 => some (['1'])
+  | Term.bvar 2 => some (['2'])
+  | Term.bvar 3 => some (['3'])
+  | Term.bvar 4 => some (['4'])
+  | Term.bvar 5 => some (['5'])
+  | Term.bvar 6 => some (['6'])
+  | Term.bvar _ => none
   | Term.fvar _ => none -- Return None immediately when an fvar is met
   | Term.abs t =>
     match encode t with
-    | some bs => some (false :: false :: bs)
+    | some bs => some ('L':: bs)
     | none => none
   | Term.app t₁ t₂ =>
     match encode t₁, encode t₂ with
-    | some bs₁, some bs₂ => some (false :: true :: bs₁ ++ bs₂)
+    | some bs₁, some bs₂ => some ('A' :: bs₁ ++ bs₂)
     | _, _ => none
 
--- 3. Decoder
-def decodeVar : List Bool → Option (Nat × List Bool)
-  | true :: false :: rest => some (0, rest)
-  | true :: true :: rest =>
-    match decodeVar (true :: rest) with
-    | some (n, rest') => some (n + 1, rest')
-    | none => none
-  | _ => none
-
-def decodeFuel : Nat → List Bool → Option (Term String × List Bool)
+@[simp, scoped grind =]
+def decodeFuel : Nat → List Char → Option (Term String × List Char)
   | 0,  _ => none
-  | f + 1, false :: false :: bs =>
+  | f + 1, 'L' :: bs =>
     match decodeFuel f bs with
     | some (t, rest) => some (Term.abs t, rest)
     | none => none
-  | f + 1, false :: true :: bs =>
+  | f + 1, 'A' :: bs =>
     match decodeFuel f bs with
     | some (t₁, rest₁) =>
       match decodeFuel f rest₁ with
       | some (t₂, rest₂) => some (Term.app t₁ t₂, rest₂)
       | none => none
     | none => none
-  | _ + 1, true :: bs =>
-    match decodeVar (true :: bs) with
-    | some (n, rest) => some (Term.bvar n, rest)
-    | none => none
+  | _ + 1, '0' :: bs => some (Term.bvar 0, bs)
+  | _ + 1, '1' :: bs => some (Term.bvar 1, bs)
+  | _ + 1, '2' :: bs => some (Term.bvar 2, bs)
+  | _ + 1, '3' :: bs => some (Term.bvar 3, bs)
+  | _ + 1, '4' :: bs => some (Term.bvar 4, bs)
+  | _ + 1, '5' :: bs => some (Term.bvar 5, bs)
+  | _ + 1, '6' :: bs => some (Term.bvar 6, bs)
   | _, __=> none
 
-def decode (bs : List Bool) : Option (Term String × List Bool) :=
+@[simp, scoped grind =]
+def decode (bs : List Char) : Option (Term String × List Char) :=
   decodeFuel bs.length bs
 
 -- 4. Auxiliary Core Properties
 
-theorem decodeVar_correct (n : Nat) (rest : List Bool) :
-    decodeVar (encodeVar n ++ rest) = some (n, rest) := by
-  induction n with
-  | zero => rfl
-  | succ m ih =>
-    cases m with
-    | zero => rfl
-    | succ k =>
-      dsimp [encodeVar, decodeVar]
-      have h : decodeVar (true :: encodeVar k ++ rest) = some (k + 1, rest) := ih
-      simp at h
-      rw [h]
-
-theorem decodeFuel_encodeVar (f n : Nat) (rest : List Bool) :
-    decodeFuel (f + 1) (encodeVar n ++ rest) = some (Term.bvar n, rest) := by
-  cases n with
-  | zero => dsimp [encodeVar, decodeFuel, decodeVar]
-  | succ m =>
-    cases m with
-    | zero => dsimp [encodeVar, decodeFuel, decodeVar]
-    | succ k =>
-      unfold decodeFuel
-      have h : decodeVar (encodeVar (k + 2) ++ rest) = some (k + 2, rest) :=
-        decodeVar_correct (k + 2) rest
-      simp [Nat.add_assoc]
-      set x := encodeVar (k + 2) ++ rest
-      split
-      any_goals tauto
-      all_goals split
-      any_goals split
-      any_goals grind
-      . rename_i heq _ _ _ _
-        rw [heq] at h
-        dsimp [decodeVar] at h
-        cases h
-      . rename_i heq _ _
-        rw [heq] at h
-        dsimp [decodeVar] at h
-        cases h
-      . rename_i heq _ _ _ _ _ _ _ _
-        rw [heq] at h
-        dsimp [decodeVar] at h
-        cases h
-      . rename_i heq _ _ _ _ _ _
-        rw [heq] at h
-        dsimp [decodeVar] at h
-        cases h
-      . rename_i heq _ _
-        rw [heq] at h
-        dsimp [decodeVar] at h
-        cases h
-
-theorem termNodes_lt_encode_length  (t : Term String) (bs : List Bool)
+theorem termNodes_lt_encode_length  (t : Term String) (bs : List Char)
     (henc : encode t = some bs) : fokker_size t < bs.length := by
   induction t generalizing bs with
-  | bvar n =>
-    simp [encode] at henc; subst bs
-    have h : (encodeVar n).length = n + 2 := by
-      induction n with | zero => rfl | succ m ih => dsimp [encodeVar]; omega
-    dsimp [fokker_size]; omega
+  | bvar n => unfold encode at henc
+              split at henc <;> grind
   | fvar x => simp [encode] at henc
   | abs body ih =>
     dsimp [encode] at henc
@@ -149,14 +100,17 @@ theorem termNodes_lt_encode_length  (t : Term String) (bs : List Bool)
 
 -- 5. Correctness Proof: `decode (encode t) = t`
 
-theorem decodeFuel_encode (t : Term String) (fuel : Nat) (bs rest : List Bool)
+theorem decodeFuel_encode (t : Term String) (fuel : Nat) (bs rest : List Char)
     (henc : encode t = some bs) (hnodes : fokker_size t < fuel) :
     decodeFuel fuel (bs ++ rest) = some (t, rest) := by
   induction t generalizing fuel bs rest with
   | bvar n =>
     cases fuel with | zero => contradiction | succ f =>
-    simp [encode] at henc; subst bs
-    rw [decodeFuel_encodeVar]
+    unfold encode at henc
+    split at henc
+    any_goals cases henc
+    any_goals simp [decodeFuel]
+    all_goals grind
   | fvar x => simp [encode] at henc
   | abs body ih =>
     cases fuel with | zero => contradiction | succ f =>
@@ -165,7 +119,7 @@ theorem decodeFuel_encode (t : Term String) (fuel : Nat) (bs rest : List Bool)
     | none => simp [h_enc] at henc
     | some bs' =>
       simp [h_enc] at henc; subst bs
-      dsimp [decodeFuel]
+      simp [decodeFuel]
       have hf : fokker_size body < f := by simp [fokker_size] at hnodes; omega
       have h1 := ih f bs' rest h_enc hf
       rw [h1]
@@ -179,8 +133,7 @@ theorem decodeFuel_encode (t : Term String) (fuel : Nat) (bs rest : List Bool)
       | none => simp [h2] at henc
       | some bs₂ =>
         simp [h1, h2] at henc; subst bs
-        dsimp [decodeFuel]
-        rw [List.append_assoc]
+        simp [decodeFuel]
         have hf₁ : fokker_size t₁ < f := by simp [fokker_size] at hnodes; omega
         have h1' := ih₁ f bs₁ (bs₂ ++ rest) h1 hf₁
         rw [h1']
@@ -198,97 +151,43 @@ theorem decode_correct (t : Term String) (bs):
   simp at h
   exact h
 
-theorem encode_wf_succeeds (t : Term String) (ht : t.fv = ∅): ∃ bs, encode t = some bs := by
+theorem encode_wf_succeeds (t : Term String) (ht : t.fv = ∅) (h7: lt7 t):
+ ∃ bs, encode t = some bs := by
 induction t with
-| bvar _ => tauto
+| bvar a => unfold encode
+            split <;> grind
 | fvar _ => simp [fv] at ht
 | abs _ _ => grind [fv, encode]
 | app _ _ ih1 ih2 =>  unfold fv at ht
                       simp at ht
                       obtain ⟨h1, h2⟩ := ht
-                      obtain ⟨_, h1⟩ := ih1 h1
-                      obtain ⟨_, h2⟩ := ih2 h2
+                      obtain ⟨_, h1⟩ := ih1 h1 (by grind)
+                      obtain ⟨_, h2⟩ := ih2 h2 (by grind)
                       unfold encode
                       simp [h1, h2]
 
 -- 6. Inverse Correctness Proof: `encode (decode bs) = bs`
 
-theorem decodeVar_sound : ∀ (bs : List Bool) (n : Nat) (rest : List Bool),
-    decodeVar bs = some (n, rest) → encodeVar n ++ rest = bs
-  | true :: false :: bs', 0, rest, h => by  simp [decodeVar] at h
-                                            subst_vars
-                                            rfl
-  | true :: true :: bs', m + 1, rest, h => by
-    simp [decodeVar] at h
-    cases h_dec : decodeVar (true :: bs') with
-    | none => simp [h_dec] at h
-    | some pair =>
-      cases pair with | mk m' r' =>
-      simp [h_dec] at h; have ⟨h1, h2⟩ := h; subst_vars
-      have ih := decodeVar_sound (true :: bs') _ _ h_dec
-      dsimp [encodeVar]; rw [ih]
-  | [], _, _, h => by contradiction
-  | [true], _, _, h => by contradiction
-  | false :: _, _, _, h => by contradiction
-  | true :: false :: _, m + 1, _, h => by simp [decodeVar] at h
-  | true :: true :: _, 0, _, h => by
-    simp [decodeVar] at h
-    rename_i tail _
-    split at h <;> cases h
-termination_by bs n rest _ => bs.length
-
-theorem decodeFuel_sound : ∀ fuel bs t rest,
+theorem decodeFuel_sound (fuel):
+     ∀ bs t rest,
     decodeFuel fuel bs = some (t, rest) →
-    ∃ t_bs, encode t = some t_bs ∧ t_bs ++ rest = bs
-  | 0, _, _,  _, h => by contradiction
-  | f + 1, false :: false :: bs, t, rest, h => by
-    simp [decodeFuel] at h
-    cases h_dec : decodeFuel f bs with
-    | none => simp [h_dec] at h
-    | some pair =>
-      cases pair with | mk t' rest' =>
-      simp [h_dec] at h; have ⟨h1, h2⟩ := h; subst_vars
-      have ⟨t_bs, henc, h_append⟩ := decodeFuel_sound f bs t' _ h_dec
-      use (false :: false :: t_bs)
-      refine ⟨by dsimp [encode]; rw [henc], by dsimp; rw [h_append]⟩
-  | f + 1, false :: true :: bs, t, rest, h => by
-    simp [decodeFuel] at h
-    cases h1 : decodeFuel f bs with
-    | none => simp [h1] at h
-    | some pair1 =>
-      cases pair1 with | mk t1 rest1 =>
-      simp [h1] at h
-      cases h2 : decodeFuel f rest1 with
-      | none => simp [h2] at h
-      | some pair2 =>
-        cases pair2 with | mk t2 rest2 =>
-        simp [h2] at h; have ⟨hx, hy⟩ := h; subst_vars
-        have ⟨t_bs1, henc1, h_app1⟩ := decodeFuel_sound f bs t1 rest1 h1
-        have ⟨t_bs2, henc2, h_app2⟩ := decodeFuel_sound f rest1 t2 _ h2
-        use (false :: true :: t_bs1 ++ t_bs2)
-        have henc_app : encode (Term.app t1 t2) = some (false :: true :: t_bs1 ++ t_bs2) := by
-          dsimp [encode]; rw [henc1, henc2]
-        refine ⟨henc_app, ?_⟩
-        subst bs
-        subst rest1
-        simp
-  | f + 1, true :: bs, t, rest, h => by
-    simp [decodeFuel] at h
-    cases h_dec : decodeVar (true :: bs) with
-    | none => simp [h_dec] at h
-    | some pair =>
-      cases pair with | mk n r =>
-      simp [h_dec] at h
-      obtain ⟨_, _⟩ := h
-      subst_vars
-      unfold encode
-      use (encodeVar n)
-      have h_sound := decodeVar_sound _ _ _ h_dec
-      tauto
-  | f + 1, [], _, _, h => by contradiction
-  | f + 1, [false], _, _, h => by contradiction
+    ∃ t_bs, encode t = some t_bs ∧ t_bs ++ rest = bs := by
+induction fuel with
+| zero => grind
+| succ n ih =>
+intros bs t rest h
+unfold decodeFuel at h
+split at h
+any_goals tauto
+any_goals split at h
+any_goals tauto
+any_goals split at h
+any_goals tauto
+any_goals cases h
+all_goals unfold encode
+all_goals grind
 
-theorem encode_decode (bs : List Bool) (t : Term String) (rest : List Bool) :
+theorem encode_decode (bs : List Char) (t : Term String) (rest : List Char) :
     decode bs = some (t, rest) →
     ∃ t_bs, encode t = some t_bs ∧ t_bs ++ rest = bs := by
   intro h
