FokkerChallenge/EncoderDecoder/Decode.lean
@@ -8,18 +8,11 @@ import FokkerChallenge.EnhancedCslib.CountBvar
 import FokkerChallenge.EnhancedCslib.Fmt
 import FokkerChallenge.EncoderDecoder.Basic
 
-def stringToBits (s : String) : List Bool := do
-  s.toList.foldr
-    (fun c acc => match c with
-                  | '0' => (false :: acc)
-                  | '1' => (true :: acc)
-                  | _   => (acc)
-    )
-    []
-
 def main (args : List String) : IO Unit := do
   for arg in args do
-    let arg := stringToBits arg
-    match Cslib.LambdaCalculus.LocallyNameless.Untyped.Term.decode arg with
+    let arg := arg.toUpper
+    let arg := arg.replace "TERM_"  ""
+    let arg := arg.replace "NORMAL_" ""
+    match Cslib.LambdaCalculus.LocallyNameless.Untyped.Term.decode arg.toList with
     | some t => IO.println s!"decoded: {t}"
     | none => IO.println "invalid BLC bitstring"
